proof/spec/xmss/XMSS_Util.ec
@@ -1,0 +1,100 @@
+pragma Goals : printall.
+
+require import AllCore List Distr RealExp IntDiv.
+require import BitEncoding.
+(*---*) import BitChunking.
+
+from Jasmin require import JModel.
+
+require import XMSS_Types.
+require import Array8.
+
+op BytesToBits (bytes : W8.t list) : bool list = flatten (map W8.w2bits bytes).
+op BitsToBytes (bits : bool list) : W8.t list = map W8.bits2w (chunk W8.size bits).
+op W64ToBytes (w : W64.t, outlen : int) : W8.t list. (* = BitsToBytes (W64.w2bits w). *)
+
+op addr_to_bytes (a : W32.t Array8.t) : W8.t list = 
+  let addr_bits : bool list = flatten (mkseq (fun (i : int) => W32.w2bits a.[i]) 8) in
+  BitsToBytes addr_bits.
+
+
+pred is_even (x : int) = x %% 2 = 0.
+
+op _ceil_2 (a : int) : int = 
+  if is_even a 
+  then to_uint (W64.of_int a `>>` W8.one) 
+  else to_uint (W64.of_int a `>>` W8.one) + 1.
+
+op _floor_2 (a : int) : int = 
+  to_uint (W64.of_int a `>>` W8.one).
+
+op nbytexor(a b : nbytes) : nbytes = 
+    map (fun (ab : W8.t * W8.t) => ab.`1 `^` ab.`2) (zip a b).
+
+lemma shr_1 (x : W64.t) :
+    to_uint (x `>>` W8.one) = to_uint x %/ 2
+        by rewrite shr_div (: (to_uint W8.one %% 64) = 1) 1:#smt:(@W64) //=. 
+
+lemma size_nbyte_xor (a b : nbytes) :
+    size a = size b =>
+      size (nbytexor a b) = size a
+        by rewrite /nbytexor size_map size_zip /#. 
+
+(******************************************************************************)
+
+(* gets the n most significant bits *)
+op msb (x : W8.t list) (n : int) : W8.t list = take n x. 
+
+(* gets the n most significant bits of x *)
+(* n is at most 32 *)
+op msb_w32 (x : W32.t) (n : int) : bool list = take n (w2bits x).
+
+(* Returns the n most significant bits of x as a W32.t *)
+op msb_w32_int (x : W32.t) (n : int) : W32.t = 
+  let bits : bool list = take n (w2bits x) in
+  (W32.bits2w bits).
+
+op lsb_w32_int (x : W32.t) (n : int) : W32.t =
+   let bits : bool list =  w2bits x in
+   let lsbits : bool list =  drop ((size bits) - n) bits in
+   W32.bits2w lsbits.
+
+(******************************************************************************)
+
+(* Stack operations *)
+op push (x : 'a list) (a : 'a) : 'a list = rcons x a. 
+
+op remove_last (x : 'a list) : 'a list = 
+with x = [] => []
+with x = h::t => if t = [] then [] else remove_last t.
+
+op pop (x : 'a list) : 'a list * 'a = 
+    let last_elem = last witness x in
+    let new_list = remove_last x in
+    (new_list, last_elem).
+
+(******************************************************************************)
+
+module Util = {
+  proc w64_to_bytes (in_0 : W64.t, outlen : int) = {
+    var r : W8.t list <- nseq outlen W8.zero;
+    var i : int;
+    var t : W8.t;
+
+    i <- outlen - 1;
+
+    while (0 <= i) {
+      t <- (truncateu8 in_0);            (* Get the lowest 8 bits *)
+      r <- put r i t;
+      in_0 <- (in_0 `>>` (W8.of_int 8)); (* Shift right by 8 bits *)
+      i <- i - 1;                        (* Move to the next byte *)
+    }
+
+    return r;
+  } 
+}.
+
+lemma w64_to_bytes_ll : 
+    phoare [Util.w64_to_bytes : 0 <= outlen ==> true] = 1%r
+        by proc; while (#pre) (i + 1); auto => /> /#.
+
