proof/spec/xmss_mt/XMSS_MT_Commons.ec
@@ -1,0 +1,281 @@
+pragma Goals : printall.
+
+
+require import AllCore List RealExp IntDiv Distr DList.
+require (*--*) Subtype. 
+
+from Jasmin require import JModel.
+ 
+require import XMSS_MT_Types XMSS_MT_Params XMSS_MT_Notation XMSS_MT_Address XMSS_MT_Hash XMSS_MT_Primitives XMSS_MT_Wots XMSS_MT_Util.
+ 
+import OTSKeys Three_NBytes AuthPath.
+import Array8.
+
+op H : nbytes -> nbytes -> nbytes.
+op H_msg : three_n_bytes -> W8.t list -> nbytes.
+op impl_oid : W32.t.
+
+(* 4.1.5 L-Trees *)
+(* takes as input a WOTS+ public key pk and compresses it to a single 
+   n-byte value pk[0].
+*)
+module LTree = {
+  proc ltree (pk : wots_pk, address : adrs, _seed : seed) : nbytes * adrs = {
+    var pk_i : nbytes;
+    var tmp : nbytes;
+    var i : int <- witness;
+    var _len : int <- len;
+    var tree_height : int;
+
+    address <- set_tree_height address 0;
+
+    while (1 < _len) { (* Same as _len > 1 *)
+      i <- 0;
+      while (i < _floor_2 _len) {
+        address <- set_tree_index address i;
+        pk_i <- nth witness pk (2*i);
+        tmp <- nth witness pk (2*i + 1);
+        (pk_i, address) <@ Hash.rand_hash (pk_i, tmp, _seed, address);
+        pk <- put pk i pk_i;
+        i <- i + 1;
+      }
+
+      if (_len %% 2 = 1) {
+        pk_i <- nth witness pk (_len - 1);
+        pk <- put pk (_floor_2 _len) pk_i;
+      }
+
+      _len <- _ceil_2 _len;
+
+      tree_height <- get_tree_height address;
+      address <- set_tree_height address (tree_height + 1);
+    }
+
+    pk_i <- nth witness pk 0;
+
+    return (pk_i, address);
+  }
+}. 
+
+
+lemma ltree_ll : islossless LTree.ltree.
+proof.
+proc.
+islossless.
+while (true) (_len - 1); last by skip => /> /#.
+auto => />.
+while (_len <= len) (floor (_len%r / 2%r) - i).
+auto => />; call rand_hash_ll. wp. skip => /> /#. 
+auto => /> &hr ?; do split.  admit. 
+move => *; split => *. 
+  + rewrite /_floor_2 shr_1 of_uintK //= #smt:(@Real).  
+  + rewrite /_ceil_2 /is_even. 
+    rewrite shr_1 of_uintK /#. 
+qed.
+
+(**********************************************************************************************)
+
+(* It is REQUIRED that s % 2^t = 0, i.e., that the leaf at index s is a leftmost leaf of a sub-tree of height t. *)
+pred leftmost_leaf (s t : int)  = s %% 2^t = 0.
+
+(* Precondition *)
+pred treehash_p (s t : int) = s %% (1 `<<` t) <> 0.
+
+
+(* NOTE: In the Jasmin implementation, treehash (in xmss_core.c) computes both the authentication 
+         path and the resulting root node *)
+(* computation of the internal n-byte nodes of a Merkle tree *)
+(* The treeHash algorithm returns the root node of a tree of height t with the leftmost 
+   leaf being the hash of the WOTS+ pk with index s.  
+*)
+module TreeHash = {
+  (* Computes the root *)
+  proc treehash(sk : xmss_mt_sk, s t : int, address : adrs) : nbytes * adrs = {
+  var node : nbytes <- nseq n W8.zero;
+  var stack : nbytes list <- [];
+  var top_node : nbytes;
+  var pub_seed : seed <- sk.`pub_seed_sk;
+  var sk_seed : seed <- sk.`sk_seed;
+  var pk : wots_pk;
+  var i : int <- 0;
+  var tree_index, tree_height: int;
+  var heights : int list <- nseq (h %/d + 1) 0;
+  var tmp : int;
+  var offset : int <- 0;
+    
+    while (i < 2^t) {
+      (* ----------- not in the RFC ----------- *)
+      offset <- offset + 1;
+      heights <- put heights (offset - 1) 0; 
+      (* -------------------------------------- *)
+
+      address <- set_type address 0;
+      address <- set_ots_addr address (s + 1);
+
+      (* Generate the public key from the secret seed *)
+      (pk, address) <@ WOTS.pkGen(sk_seed, pub_seed, address);
+
+      address <- set_type address 1;
+      address <- set_tree_addr address (s + 1);
+
+      (node, address) <@ LTree.ltree(pk, address, pub_seed); 
+
+      address <- set_type address 2;
+      address <- set_tree_height address 0;
+      address <- set_tree_index address (i + 1);
+      
+      top_node <- last witness stack;
+
+      (* While the top-most nodes are of equal height *)
+      (* offset >= 2 <=> 2 <= offset *)
+      
+      while (2 <= offset /\ ((nth witness heights (offset - 1)) = (nth witness heights (offset - 2)))) {
+        tree_index <- get_tree_index address;
+        address <- set_tree_index address (ceil((tree_index - 1)%r / 2%r));
+        (stack, top_node) <- pop stack;
+
+        (node, address) <@ Hash.rand_hash (top_node, node, pub_seed, address);
+        
+        (* ----------- not in the RFC ----------- *)
+        offset <- offset - 1;
+        tmp <- nth witness heights (offset - 1);
+        heights <- put heights (offset - 1) (t + 1);
+        (* -------------------------------------- *)
+
+        tree_height <- get_tree_height address;
+        address <- set_tree_height address (tree_height + 1); (* Move to the next tree *)
+      }
+
+      stack <- push stack node;
+      i <- i + 1;
+    }
+    
+  return (node, address);
+  }
+}.
+
+lemma treehash_ll : islossless TreeHash.treehash.
+proof.
+proc.
+sp ; wp.
+while (true) (2^t - i); last by skip => /> /#.
+auto => />. sp.
+while (true) (offset - 1).
+  + auto => />; call rand_hash_ll; wp; skip => /> /#.
+  + wp; call ltree_ll; wp; call wots_pkGen_ll; wp. skip => /> *.
+    split; [ move => *; rewrite negb_and; left |]; smt().
+qed.
+
+module TreeSig = {
+  (* Compute the authentication path for the i-th WOTS+ key pair *)
+  proc buildAuthPath(sk : xmss_mt_sk, idx : W32.t, address : adrs) : auth_path * adrs = {
+    var authentication_path : auth_path <- nseq len (nseq n W8.zero);
+    var j : int <- 0;
+    var k : int;
+    var t : nbytes <- witness;
+
+    while (j < h) {
+      k <- floor((W32.to_uint idx)%r / (2^j)%r);
+      (t, address) <@ TreeHash.treehash(sk, k * (2^j), j, address);
+      authentication_path <- put authentication_path j t;
+      j <- j + 1;
+    }
+
+    return (authentication_path, address);
+  }
+
+  (* Generate a WOTS+ signature on a message with corresponding authentication path *)
+  proc treesig(M : nbytes, sk : xmss_mt_sk, idx : W32.t, address : adrs) : wots_signature * auth_path * adrs  = {
+    var auth : auth_path <- nseq len (nseq n W8.zero);
+    var sig_ots : wots_signature;
+    var ots_sk : wots_sk;
+    var seed : nbytes;
+    
+    (auth, address) <@ buildAuthPath (sk, idx, address);
+    address <- set_type address 0;
+    address <- set_ots_addr address (W32.to_uint idx);
+
+    (sig_ots, address) <@ WOTS.sign_seed(M, sk.`sk_seed, sk.`pub_seed_sk, address);
+    
+    return (sig_ots, auth, address);
+  }
+}.
+
+lemma buildAuthPath_ll : islossless TreeSig.buildAuthPath.
+proof.
+proc.
+while (0 <= j <= h) (h - j) ; auto => />; [call treehash_ll ; auto => /> /# | smt(h_g0) ]. 
+qed.
+
+lemma treesig_ll : islossless TreeSig.treesig
+    by proc; call wots_sign_seed_ll; auto => /> ; call buildAuthPath_ll; auto.
+
+(**********************************************************************************************)
+
+op append_sig (sig : sig_t) (r_sig : reduced_signature) : sig_t =    
+    let new_sigs: reduced_signature list = sig.`r_sigs ++ [r_sig] in
+    {| sig with  r_sigs=new_sigs|}.
+
+(**********************************************************************************************)
+
+module RootFromSig = {
+  proc rootFromSig(idx_sig : W32.t, sig_ots : wots_signature, auth : auth_path, M : nbytes, 
+  _seed : seed, address : adrs) : nbytes = {
+    var pk_ots : wots_pk;
+    var k : int;
+    var nodes0, nodes1 : nbytes;
+    var index : int;
+    var auth_k : nbytes;
+    
+    address <- set_type address 0;
+    address <- set_ots_addr address (W32.to_uint idx_sig);
+
+    (pk_ots, address) <@ WOTS.pkFromSig(M, sig_ots, _seed, address);
+
+    address <- set_type address 1;
+    address <- set_ltree_addr address (W32.to_uint idx_sig);
+
+    (nodes0, address) <@ LTree.ltree(pk_ots, address, _seed);
+
+    address <- set_type address 2;
+    address <- set_tree_index address (W32.to_uint idx_sig);
+
+    k <- 0;
+    while (k < h) {
+      address <- set_tree_height address k;
+
+      if (floor ((W32.to_uint idx_sig)%r / (2^k)%r) %% 2 = 0) {
+        index <- get_tree_index address;
+        address <- set_tree_index address (index %/ 2);
+
+        auth_k <- nth witness auth k;
+        (nodes1, address) <@ Hash.rand_hash (nodes0, auth_k, _seed, address);
+      } else {
+        index <- get_tree_index address;
+        address <- set_tree_index address ((index - 1) %/ 2);
+
+        auth_k <- nth witness auth k;
+        (nodes1, address) <@ Hash.rand_hash (auth_k, nodes0, _seed, address);
+      }
+
+      nodes0 <- nodes1;
+      k <- k+1;
+    }
+
+    return nodes0;
+  }
+}.
+
+lemma root_from_sig_ll : islossless RootFromSig.rootFromSig.
+proof.
+proc.
+while (0 <= k <= h) (h - k) ; auto => />.
+  + wp; sp. if. 
+      * call rand_hash_ll. islossless. auto => /> &hr *; do split; admit. 
+      * call rand_hash_ll. islossless. auto => /> &hr *; do split; admit.
+  + auto => />; do split => /#.
+  + call ltree_ll ; auto => />. 
+    call wots_pkFromSig_ll ; auto => />.
+    smt(h_g0).
+qed.
+
