proof/spec/xmss_mt/XMSS_MT_Hash.ec
@@ -6,7 +6,7 @@ require import BitEncoding.
 
 from Jasmin require import JModel.
 
-require import Types Params Util (* Utils *) Address.
+require import XMSS_MT_Types XMSS_MT_Params XMSS_MT_Util XMSS_MT_Address.
 
 op Hash : W8.t list -> W8.t list.
 
