proof/spec/xmss_mt/XMSS_MT_Notation.ec
@@ -1,0 +1,65 @@
+pragma Goals : printall.
+
+require import AllCore List RealExp IntDiv.
+
+from Jasmin require import JModel.
+
+require import XMSS_MT_Params.
+
+(* prefix of big endian byte representation of a 32-bit word *)
+op toByte(x : W32.t, k : int) : W8.t list =  
+     take k (rev (to_list (W4u8.unpack8 x))).
+
+(* From the RFC
+  A byte string can be considered as a string of base w numbers, i.e.,
+  integers in the set {0, ... , w - 1}.
+  In base_w(X, w, out_len), the length out_len is REQUIRED to be less than 
+  or equal to 8 * len_X / lg(w).
+*)
+module BaseW = {
+  proc base_w(X : W8.t list, outlen : int) : int list = {
+    var _in : int <- 0;
+    var out : int <- 0;
+    var total : W8.t <- W8.zero;
+    var bits : int <- 0;
+    var consumed : int <- 0;
+    var base_w : int list;
+    var v : int;
+
+    base_w <- nseq outlen 0;
+
+    while (consumed < outlen) {
+      if (bits = 0) {
+        total <- nth witness X _in;
+        _in <- _in + 1;
+        bits <- bits + 8;
+      }
+
+      bits <- bits - floor(log2 w%r);
+      
+      v <- (W8.to_uint ((total `>>` W8.of_int bits) `&` W8.of_int (w - 1)));
+      base_w <- put base_w out v;
+
+      out <- out + 1;
+      consumed <- consumed + 1;
+    }
+    
+    return base_w;
+  }
+}.
+
+pred base_w_pre (X : W8.t list, outlen : int) =
+  0 <= outlen <= 8 * size X %/ floor (log2 w%r).
+
+pred base_w_post (X : W8.t list, outlen : int, base_w : int list) =
+  size base_w = outlen /\
+  all (fun x => 0 <= x <= w - 1) base_w.
+
+axiom base_w_pre_post : hoare [BaseW.base_w : base_w_pre X outlen ==> true (* base_w_post X outlen res *)].
+
+lemma base_w_spec_ll : islossless BaseW.base_w.
+proof.
+proc ; while (true) (outlen - consumed) ; auto => /> /#.
+qed.
+
+
