proof/spec/xmss_mt/XMSS_MT_Types.ec
@@ -1,0 +1,76 @@
+require import AllCore List RealExp IntDiv.
+require (*  *) Subtype. 
+
+require import XMSS_Params.
+
+from Jasmin require import JModel.
+
+require import Array8.
+
+type adrs = W32.t Array8.t.
+
+type nbytes = W8.t list. (* size = n *)
+type len_n_bytes = nbytes list. (* list of length len, each element of length n *)
+type len1_bytes = W8.t list. (* list of length len1 *)
+
+(******************************************************************************)
+
+type key = nbytes.
+type seed = nbytes.
+
+(******************************************************************************)
+
+type wots_message = nbytes.
+type wots_message_base_w = len1_bytes.
+type wots_signature = len_n_bytes.
+type wots_pk = len_n_bytes.
+type wots_sk = len_n_bytes.
+type wots_keypair = wots_pk * wots_sk.
+
+(******************************************************************************)
+
+clone import Subtype as OTSKeys with 
+   type T = wots_sk list,
+   op P = fun l => size l = 2^h
+   rename "T" as "wots_ots_keys".
+
+clone import Subtype as Three_NBytes with 
+   type T = W8.t list,
+   op P = fun l => size l = 3 * n
+   rename "T" as "three_n_bytes"
+   proof inhabited by (exists (nseq (3*n) W8.zero);smt(size_nseq ge0_n))
+   proof *.
+
+(* treeheight . n *)
+clone import Subtype as AuthPath with
+  type T = nbytes list,
+  op P = fun l => size l = d
+  rename "T" as "auth_path"
+  proof inhabited by admit
+  proof *.
+
+(******************************************************************************)
+
+(* Same as single tree variant *)
+type xmss_mt_sk = { idx : W32.t ;
+                    sk_seed : nbytes ; (* secret *)
+                    sk_prf : nbytes ;
+                    pub_seed_sk : nbytes ; (* public *)
+                    sk_root : nbytes }.
+
+(* Same as single tree variant *)
+type xmss_mt_pk = { pk_oid : W32.t ;
+                    pk_root : nbytes ;
+                    pk_pub_seed : nbytes }.
+
+type msg_t = W8.t list.
+
+type reduced_signature = wots_signature * auth_path.
+
+type sig_t = { sig_idx : W32.t;
+               r : nbytes ;
+               r_sigs : reduced_signature list }.
+
+type xmss_mt_keypair = xmss_mt_sk * xmss_mt_pk.
+
+(******************************************************************************)
